Engine/Correctness.v
@@ -9,7 +9,7 @@ From Linden Require Import NFA PikeTree PikeVM.
 From Linden Require Import PikeEquiv PikeSubset.
 From Linden Require Import EquivMain RegexpTranslation GroupMapMS.
 From Linden Require Import ResultTranslation FunctionalUtils SeenSets.
-From Linden Require Import Parameters.
+From Linden Require Import Parameters Prefix.
 From Warblre Require Import Base Semantics Result RegExpRecord StaticSemantics.
 Import Result.Notations.
 
@@ -38,21 +38,21 @@ Qed.
 Section Correctness.
   Context {params: LindenParameters}.
   Context {VMS: VMSeen}.
+  Context {strs: StrSearch}.
   Context (rer: RegExpRecord).
 
 Definition trc_pike_tree := @trc pike_tree_state pike_tree_step.
-Definition trc_pike_vm (c:code) := @trc pike_vm_state (pike_vm_step rer c).
-
+Definition trc_pike_vm (c:code) (lit:literal) := @trc pike_vm_state (pike_vm_step rer c lit).
 
 (* The Pike invariant is preserved through the TRC *)
 Lemma vm_to_tree:
-  forall svm1 st1 svm2 code
+  forall svm1 st1 svm2 code lit
     (STWF: stutter_wf rer code)
     (INVARIANT: pike_inv rer code st1 svm1)
-    (TRCVM: trc_pike_vm code svm1 svm2),
+    (TRCVM: trc_pike_vm code lit svm1 svm2),
     exists st2, trc_pike_tree st1 st2 /\ pike_inv rer code st2 svm2.
 Proof.
-  intros svm1 st1 svm2 code STWF INVARIANT TRCVM.
+  intros svm1 st1 svm2 code lit STWF INVARIANT TRCVM.
   generalize dependent st1. induction TRCVM; intros.
   { exists st1. split; auto. apply trc_refl. }
   eapply invariant_preservation in STEP; eauto.
@@ -65,13 +65,13 @@ Qed.
 
 (* Any execution of the PikeVM to a final state corresponds to an execution of the PikeTree *)
 Theorem pike_vm_to_pike_tree:
-  forall r inp tree result,
+  forall r lit inp tree result,
     pike_regex r -> 
     bool_tree rer [Areg r] inp CanExit tree ->
-    trc_pike_vm (compilation r) (pike_vm_initial_state inp) (PVS_final result) ->
+    trc_pike_vm (compilation r) lit (pike_vm_initial_state inp) (PVS_final result) ->
     trc_pike_tree (pike_tree_initial_state tree inp) (PTS_final result).
 Proof.
-  intros r inp tree result SUBSET TREE TRCVM.
+  intros r lit inp tree result SUBSET TREE TRCVM.
   generalize (initial_pike_inv rer r inp tree (compilation r) TREE (@eq_refl _ _) SUBSET).
   intros INIT.
   eapply vm_to_tree in TRCVM as [vmfinal [TRCTREE INV]]; eauto.
@@ -95,17 +95,17 @@ Qed.
 (** * Correctness Theorem of the PikeVM result  *)
 
 Theorem pike_vm_correct:
-  forall r inp tree result,
+  forall r lit inp tree result,
     (* the regex `r` is in the supported subset *)
     pike_regex r ->
     (* `tree` is the tree of the regex `r` for the input `inp` *)
     is_tree rer [Areg r] inp GroupMap.empty forward tree ->
     (* the result of the PikeVM is `result` *)
-    trc_pike_vm (compilation r) (pike_vm_initial_state inp) (PVS_final result) ->
+    trc_pike_vm (compilation r) lit (pike_vm_initial_state inp) (PVS_final result) ->
     (* This `result` is the priority result of the `tree` *)
     result = first_leaf tree inp.
 Proof.
-  intros r inp tree result SUBSET TREE TRC.
+  intros r lit inp tree result SUBSET TREE TRC.
   eapply encode_equal with (b:=CanExit) in TREE as BOOLTREE; pike_subset.
   eapply pike_vm_to_pike_tree in TRC; eauto.
   assert (SUBTREE: pike_subtree tree).
@@ -119,35 +119,35 @@ Qed.
 
 (* Equivalence of PikeVM to Warblre backtracking algorithm *)
 Theorem pike_vm_same_warblre:
-  forall lr wr inp,
+  forall lr lit wr inp,
     pike_regex lr ->
     equiv_regex wr lr ->
     RegExpRecord.capturingGroupsCount rer = StaticSemantics.countLeftCapturingParensWithin wr nil ->
     EarlyErrors.Pass_Regex wr nil ->
     forall result,
-      trc_pike_vm (compilation lr) (pike_vm_initial_state inp) (PVS_final result) ->
+      trc_pike_vm (compilation lr) lit (pike_vm_initial_state inp) (PVS_final result) ->
       EquivDef.equiv_res result ((EquivMain.compilePattern wr rer) (input_str inp) (idx inp)).
 Proof.
-  intros lr wr inp Hpike Hequiv Hcapcount HearlyErrors.
+  intros lr lit wr inp Hpike Hequiv Hcapcount HearlyErrors.
   pose proof equiv_main wr lr rer inp Hequiv Hcapcount HearlyErrors as HequivMain.
   destruct HequivMain as [m [res [Hcompsucc [Hexecsucc Hsameresult]]]].
   unfold compilePattern. rewrite Hcompsucc, Hexecsucc.
   set (tree := FunctionalUtils.compute_tr rer [Areg lr] inp GroupMap.empty forward).
   specialize (Hsameresult tree eq_refl). destruct Hsameresult as [His_tree Hsameresult].
   intros result Hpikeresult.
-  pose proof pike_vm_correct lr inp tree result Hpike His_tree Hpikeresult as Hsameresult'.
+  pose proof pike_vm_correct lr lit inp tree result Hpike His_tree Hpikeresult as Hsameresult'.
   rewrite Hsameresult'. assumption.
 Qed.
 
 (* Same, but with an input that is at the beginning of the input string *)
 Theorem pike_vm_same_warblre_str0:
-  forall lr wr str0,
+  forall lr lit wr str0,
     pike_regex lr ->
     equiv_regex wr lr ->
     RegExpRecord.capturingGroupsCount rer = StaticSemantics.countLeftCapturingParensWithin wr nil ->
     EarlyErrors.Pass_Regex wr nil ->
     forall result,
-      trc_pike_vm (compilation lr) (pike_vm_initial_state (init_input str0)) (PVS_final result) ->
+      trc_pike_vm (compilation lr) lit (pike_vm_initial_state (init_input str0)) (PVS_final result) ->
       EquivDef.equiv_res result ((EquivMain.compilePattern wr rer) str0 0).
 Proof.
   intros lr wr str0 Hpike Hequiv Hcapcount HearlyErrors.
@@ -157,7 +157,7 @@ Qed.
 (* Equivalence of PikeVM to Warblre Semantics *)
 (* A version closer to the paper definition *)
 Theorem pike_vm_warblre:
-  forall rw r inp result,
+  forall rw r lit inp result,
     (* For a correct RegExpRecord *)
     RegExpRecord.capturingGroupsCount rer = countLeftCapturingParensWithin rw [] ->
     (* For any Warblre regex that passes the early errors check, *)
@@ -167,11 +167,11 @@ Theorem pike_vm_warblre:
     (* such that it is in the supported PikeVM subset *)
     pike_regex r ->
     (* When PikeVM reaches a final result *)
-    trc_pike_vm (compilation r) (pike_vm_initial_state inp) (PVS_final result) ->
+    trc_pike_vm (compilation r) lit (pike_vm_initial_state inp) (PVS_final result) ->
     (* this result is equal to Warblre's execution result *)
     (compilePattern rw rer) (input_str inp) (idx inp) = to_MatchState result (RegExpRecord.capturingGroupsCount rer).
 Proof.
-  intros rw r inp result RER EARLY TOLINDEN SUBSET TRC.
+  intros rw r lit inp result RER EARLY TOLINDEN SUBSET TRC.
   specialize (earlyErrors_pass_translation _ EARLY) as [lr SUCCESS].
   unfold warblre_to_linden' in TOLINDEN. rewrite SUCCESS in TOLINDEN. subst.
   specialize (warblre_to_linden_sound_root _ _ SUCCESS) as EQUIV.
@@ -179,10 +179,9 @@ Proof.
   specialize (equiv_main _ _ _ inp EQUIV RER PASS) as [m [res [COMP_SUCC [EXEC_SUCC LW_EQUIV]]]].
   unfold compilePattern. rewrite COMP_SUCC, EXEC_SUCC.
   specialize (LW_EQUIV (compute_tr rer [Areg lr] inp GroupMap.empty forward) eq_refl) as [ISTREE LW_EQUIV].
-  specialize (pike_vm_correct _ _ _ _ SUBSET ISTREE TRC) as FIRST. subst.  
+  specialize (pike_vm_correct _ _ _ _ _ SUBSET ISTREE TRC) as FIRST. subst.  
   symmetry. apply to_MatchState_equal; auto.
   eapply compilePattern_preserves_groupcount; eauto.
 Qed.
 
 End Correctness.
-
